H10/Fractran/mm_fractran.v
@@ -1,0 +1,485 @@
+(**************************************************************)
+(*   Copyright Dominique Larchey-Wendling [*]                 *)
+(*             Yannick Forster            [+]                 *)
+(*                                                            *)
+(*                             [*] Affiliation LORIA -- CNRS  *)
+(*                             [+] Affiliation Saarland Univ. *)
+(**************************************************************)
+(*      This file is distributed under the terms of the       *)
+(*         CeCILL v2 FREE SOFTWARE LICENSE AGREEMENT          *)
+(**************************************************************)
+
+Require Import List Arith Omega Permutation.
+
+Import ListNotations.
+
+Require Import utils_tac utils_list utils_nat gcd prime rel_iter pos vec.
+Require Import sss subcode mm_defs mm_no_self.
+Require Import fractran_defs prime_seq.
+
+Set Implicit Arguments.
+
+Tactic Notation "rew" "length" := autorewrite with length_db. 
+
+Local Notation "e #> x" := (vec_pos e x).
+Local Notation "e [ v / x ]" := (vec_change e x v).
+
+Local Notation "I // s -1> t" := (mm_sss I s t).
+Local Notation "P /MM/ s → t" := (sss_step (@mm_sss _) P s t) (at level 70, no associativity). 
+Local Notation "P /MM/ s -[ k ]-> t" := (sss_steps (@mm_sss _) P k s t) (at level 70, no associativity).
+Local Notation "P /MM/ s ↓" := (sss_terminates (@mm_sss _) P s) (at level 70, no associativity).
+
+Local Notation "l /F/ x → y" := (fractran_step l x y) (at level 70, no associativity).
+Local Notation "l /F/ x -[ k ]-> y" := (fractran_steps l k x y) (at level 70, no associativity).
+
+Set Implicit Arguments.
+
+(* Fractran simulates MM *)
+
+(*       let a MM program 1: INC ... k: DEC ... n: _ *)
+(*       with variables x1...xm *)
+
+(*    we use p1...pn,q1...qm distinct primes and  *)
+(*    encode the state (i,v1,...,vm) *)
+(*    as p1^0*...*pi^1*...*pn^0*q1^v1*...*qm^vm *)
+
+(*    i: INC xu   ---> (qu*p(i+1) / pi) *)
+(*    i: DEC xu j ---> (p(i+1) / pi*qu) and (pj / pi) (the second constraint should appear AFTER in the list) *)
+
+Definition encode_state {n} (c : nat * vec nat n) := ps (fst c) * @exp n 0 (snd c).
+
+Definition encode_inc n  i (u : pos n) := (ps (i + 1) * qs u, ps i).
+Definition encode_dec n  i (u : pos n) (_ : nat) := (ps (i + 1), ps i * qs u).
+Definition encode_dec2 n i (u : pos n) j := (ps j, ps i).
+
+Fixpoint encode_mm_instr m i (l : list (mm_instr m)) : list (nat * nat) :=
+  match l with
+  | nil          => nil
+  | INC u   :: l => encode_inc i u                        :: encode_mm_instr (S i) l
+  | DEC u j :: l => encode_dec i u j :: encode_dec2 i u j :: encode_mm_instr (S i) l
+  end.
+
+Fact encode_mm_instr_regular n i l : Forall (fun c => fst c <> 0 /\ snd c <> 0) (@encode_mm_instr n i l).
+Proof.
+  revert i; induction l as [ | [ u | u j ] l IHl ]; intros i; simpl.
+  + constructor.
+  + constructor; auto; unfold encode_inc; simpl; split;
+      [ apply Nat.neq_mul_0; split | ]; apply prime_neq_0; apply nthprime_prime.
+  + constructor; [ | constructor ]; auto; split; unfold encode_dec, encode_dec2; simpl.
+    2: apply Nat.neq_mul_0; split.
+    all: apply prime_neq_0; apply nthprime_prime.
+Qed.
+
+Local Notation divides_mult_inv := prime_div_mult.
+
+Local Ltac inv H := inversion H; subst; clear H.
+
+Opaque ps qs.
+
+Lemma divides_encode_state i k n v : divides (ps i) (@encode_state n (k,v)) -> i = k.
+Proof.
+  unfold encode_state. intros. induction v.
+  - cbn in H. replace (ps k * 1) with (ps k) in H by omega.
+    now eapply primestream_divides in H.
+  - cbn in H. eapply divides_mult_inv in H as [ | [ | ] % divides_mult_inv ]; eauto.
+    + now eapply primestream_divides in H.
+    + eapply divides_pow in H; eauto.
+      now eapply ps_qs_div in H.
+    + now eapply ps_exp in H.
+Qed.
+
+Lemma skip_steps m k l r k' (v v' : vec _ m) :
+      @mm_no_self_loops m (k, l ++ r) 
+   -> encode_mm_instr (k + length l) r /F/ encode_state (k + length l,v) → encode_state (k',v') 
+   -> encode_mm_instr k (l ++ r)       /F/ encode_state (k + length l,v) → encode_state (k',v').
+Proof with eauto; try omega.
+  revert k. induction l; cbn - [subcode] in *; intros.
+  - revert H0. ring_simplify (k + 0). eauto.
+  - revert H0. ring_simplify (k + S (length l)). intros H1. destruct a.
+    + econstructor 2. intros [[|] % divides_mult_inv | ] % divides_mult_inv; eauto.
+      * eapply primestream_divides in H0; omega.
+      * now eapply ps_qs_div in H0. 
+      * eapply divides_encode_state in H0; omega.
+      * specialize IHl with (k := S k). revert IHl.
+        cbn - [subcode]. ring_simplify (S (k + length l)).
+        intros IHl. eapply IHl. 2:exact H1.
+        intros ? ? ?. eapply H. eapply subcode_cons. eassumption.
+    + repeat econstructor 2. 2:unfold encode_dec2.
+      2,3: cbn- [subcode]. 1: intros [] % divides_mult_inv_l.
+      2: intros [ | ] % divides_mult_inv...
+      * eapply divides_mult_inv in H0 as [? | ?]...
+        eapply primestream_divides in H0...
+        eapply divides_encode_state in H0... 
+      * eapply primestream_divides in H0... subst.
+        eapply (H n p). eauto.
+      * eapply divides_encode_state in H0...
+      * specialize (IHl (S k)). revert IHl.
+        cbn - [subcode]. ring_simplify (S (k + length l)).
+        intros IHl. eapply IHl. 2:exact H1.
+        intros ? ? ?. eapply H. eapply subcode_cons. eassumption.
+Qed.
+
+Lemma qs_exp i n u (v : vec nat n) :
+  divides (qs u) (encode_state (i,v)) <-> divides (qs u) (exp 0 v).
+Proof.
+  split.
+  - intros [ | ] % divides_mult_inv; eauto.
+    now eapply qs_ps_div in H.
+  - intros. unfold encode_state. now eapply divides_mult.
+Qed.
+
+Lemma qs_encode_state i n (u : pos n) (v : vec nat n) :
+  divides (qs u) (encode_state (i,v)) <-> v #> u > 0.
+Proof.
+  rewrite qs_exp.
+  enough (forall i, divides (qs (i + u)) (exp i v) <-> v #> u > 0). eapply H. intros j.
+  induction v.
+  - inversion u.
+  - revert u. eapply pos.pos_S_invert.
+    + cbn; rewrite pos2nat_fst, Nat.add_0_r. 
+      split.
+      * intros [ | ] % divides_mult_inv; eauto.
+        -- destruct x; try omega. cbn in H. 
+           apply divides_1_inv in H.
+           generalize (str_prime qs j); rewrite H.
+           intros [ [] _ ]; auto.
+        -- eapply qs_exp_div in H; now eauto.
+      * intros. destruct x. inv H.
+        exists (qs j ^ x * exp (S j) v). cbn. ring.
+    + cbn. intros. rewrite <- IHv, pos2nat_nxt.
+      rewrite qs_shift with (m := 1).
+      simpl.
+      replace (j+S (pos2nat p)) with (S (j+p)); try tauto.
+      2: rewrite (plus_comm _ (S _)); simpl; rewrite plus_comm; auto.
+      split; intros H.
+      * eapply divides_mult_inv in H as [ | ]; eauto.
+        eapply divides_pow in H; auto. 
+        eapply primestream_divides in H.
+        omega.
+      * eapply divides_mult. 
+        revert H; cbn; rewrite plus_n_Sm; eauto.
+Qed.
+
+Lemma one_step_forward m i P i1 v1 i2 v2 :
+     @mm_no_self_loops m (i,P) 
+  -> (i, P)              /MM/ (i1, v1)           → (i2,v2) 
+  -> encode_mm_instr i P /F/  encode_state (i1,v1) → encode_state (i2,v2).
+Proof with eauto; try omega.
+  intros HP (k & l & [ u | u j ] & r & v & ? & ? & ?); inversion H; subst; clear H.
+  - inversion H0; inversion H1; subst; clear H0 H1. 
+    eapply skip_steps...
+    econstructor. cbn. ring_simplify.
+    replace (1 + (k + length l)) with (k + length l + 1) by omega. unfold encode_state, fst, snd. 
+    rewrite vec_prod_mult.
+    rewrite Nat.add_0_r; ring.
+  - inversion H0; inversion H1; subst; clear H0 H1.
+    all:eapply skip_steps...
+    + cbn. econstructor 2.
+      intros [] % divides_mult_inv_l...
+      eapply divides_mult_inv in H0 as [ | ]...
+      * now eapply qs_ps_div in H0.          
+      * eapply qs_encode_state in H0. omega.
+      * unfold encode_dec2. econstructor. unfold encode_state, fst, snd. ring.
+    + econstructor. cbn. unfold encode_state, fst, snd. ring_simplify.
+      replace (1 + (k + length l)) with (k + length l + 1) by omega.
+      erewrite <- (vec_prod_div _ _ _ H4).
+      rewrite Nat.add_0_r; ring.
+Qed.
+
+Lemma steps_forward m i P i1 v1 i2 v2 k :
+    @mm_no_self_loops m (i, P) 
+ -> (i, P) /MM/ (i1, v1) -[k]-> (i2,v2)
+ -> encode_mm_instr i P /F/ encode_state (i1,v1) -[k]-> encode_state (i2,v2).
+Proof.
+  intros HP H. revert v1 i1 i2 H. induction k; intros v1 i1 i2 H; inversion H; subst; clear H; cbn.
+  - reflexivity.
+  - destruct st2. eapply one_step_forward in H1; eauto.
+Qed.
+
+Ltac list_without L v :=
+  match L with
+  | ?L * v => list_without L v
+  | v * ?L => list_without L v
+  | ?L * ?R => let l := list_without L v in
+              let r := list_without R v in constr:(l * r)
+  | ?L => constr:(L)
+  end.
+
+Ltac factorout H v :=
+  match type of H with ?L = ?R =>
+                       let L := list_without L v in
+                       let R := list_without R v in
+                       let H' := fresh "H" in
+                       rename H into H';
+                       assert (H : L = R); [ eapply Nat.mul_cancel_l with v; [ eauto | ring_simplify; ring_simplify in H'; (rewrite H' || rewrite <- H'); ring] | ]; clear H'
+  end.
+
+Lemma mm_no_self_loops_cons n i a P : mm_no_self_loops   (i, a :: P) 
+                                  -> @mm_no_self_loops n (1 + i, P).
+Proof.
+  intros ? ? ? ?. 
+  eapply (H i0 x). 
+  now eapply subcode_cons.
+Qed. 
+
+Hint Resolve mm_no_self_loops_cons.
+
+Lemma one_step_backward m i P i1 v1 i2 v2 :
+     @mm_no_self_loops m (i, P) 
+  -> encode_mm_instr i P /F/  encode_state (i1,v1) → encode_state (i2,v2)
+  ->              (i, P) /MM/ (i1, v1)           → (i2,v2).
+Proof with eauto; try omega.
+  revert i i1 i2 v1 v2.  induction P; intros i i1 i2 v1 v2 HP H; cbn; inv H.
+  all: destruct a; inv H0. all:unfold encode_state, fst, snd in *. all: try ring_simplify in H1.
+  all: try ring_simplify in H2.
+  - assert (i = i1) as ->. {
+      match type of H1 with _ = ?r => assert (divides (ps i) r) end.
+      rewrite <- H1. exists (ps i2 * exp 0 v2). ring.
+      eapply divides_mult_inv in H as [[[ | ] % divides_mult_inv | ] % divides_mult_inv | ]...
+      + eapply primestream_divides in H. omega.
+      + now eapply ps_qs_div in H.
+      + eauto using primestream_divides.
+      + now eapply ps_exp in H.
+    } ring_simplify  in H1.
+    factorout H1 (ps i1).
+    
+    assert (i2 = i1 + 1) as ->. {
+      assert (divides (ps i2) (ps (i1 + 1) * qs p0 * exp 0 v1)).
+      rewrite <- H1. exists (exp 0 v2). ring.
+      eapply divides_mult_inv in H as [[ | ] % divides_mult_inv | ]...
+      + eapply primestream_divides in H; eauto.
+      + now eapply ps_qs_div in H.
+      + now eapply ps_exp in H.
+    } clear IHP.
+
+    factorout H1 (ps (i1 + 1)).
+    rewrite <- exp_inv_inc in H1. eapply exp_inj in H1 as ->.
+    
+    exists i1,[],(INC p0), P, v1. repeat split; try f_equal.
+    cbn. omega. replace (i1 + 1) with (1 + i1) by omega. econstructor.
+  - assert (i = i1) as ->.
+    { match type of H1 with _ = ?r => assert (divides (ps i) r) end.
+      rewrite <- H1. exists (qs p0 * ps i2 * exp 0 v2). ring.
+      eapply divides_mult_inv in H as [[ | ] % divides_mult_inv | ]...
+      + eapply primestream_divides in H...
+      + eapply primestream_divides in H...
+      + eapply ps_exp in H...
+    } factorout H1 (ps i1).
+
+    assert (i2 = i1 + 1) as ->. {
+      match type of H1 with _ = ?r => assert (divides (ps i2) r) end.
+      rewrite <- H1. exists (qs p0 * exp 0 v2). ring.
+      eapply divides_mult_inv in H as [ | ]... 
+      + eapply primestream_divides in H...
+      + eapply ps_exp in H...
+    } clear IHP. factorout H1 (ps (i1 + 1)).
+    symmetry in H1. rewrite <- exp_inv_inc in H1. eapply exp_inj in H1 as ->.
+
+    eexists i1,[], (DEC p0 n), P, _. repeat split; try f_equal.
+    cbn. omega. replace (i1 + 1) with (1 + i1) by omega.
+    pose proof (@in_mm_sss_dec_1 _ i1 p0 n (vec_change v2 p0 (S (vec_pos v2 p0))) (vec_pos v2 p0)).
+    rewrite vec_change_eq in H... specialize (H eq_refl).
+    now rewrite vec_change_idem, vec_change_same in H.
+  - eapply IHP in H2. all: try now (cbn in *; omega).
+    destruct H2 as (k & l & [ u | u j ] & r & v & ? & ? & ?).
+    + inv H. inv H0. inv H2. 
+      exists i. exists (INC p0 :: l). exists (INC u). exists r. exists v.
+      cbn. repeat split. f_equal. omega.
+      econstructor.
+    + inv H. inv H0. inv H2. 
+      * exists i. exists (INC p0 :: l). exists (DEC u i2). exists r. exists v2.
+        cbn. repeat split. f_equal. omega.
+        econstructor. eauto.
+      * exists i. exists (INC p0 :: l). exists (DEC u j). exists r. exists v.
+        cbn. repeat split. f_equal. omega.
+        econstructor. eauto.
+    + eauto.
+  -  unfold encode_dec2 in H2. cbn in H2. inv H2.
+     * assert (i = i1) as ->.
+       { match type of H6 with _ = ?r => assert (divides (ps i) r) end.
+         rewrite <- H6. exists (ps i2 * exp 0 v2). ring. ring_simplify in H.
+         eapply divides_mult_inv in H as [[|] % divides_mult_inv | ]...
+         + eapply primestream_divides in H... subst.
+           edestruct (HP n p0)...
+         + eapply primestream_divides in H...
+         + eapply ps_exp in H...
+       } factorout H6 (ps i1).
+
+       assert (i2 = n) as ->. {
+         match type of H6 with _ = ?r => assert (divides (ps i2) r) end.
+         rewrite <- H6. exists (exp 0 v2). ring.
+         eapply divides_mult_inv in H as [ | ]...
+         + eapply primestream_divides in H... 
+         + eapply ps_exp in H...
+       } clear IHP.
+       rewrite Nat.mul_cancel_l in H6...
+
+       eapply exp_inj in H6 as ->.
+
+       eexists i1,[], (DEC p0 n), P, _. repeat split; try f_equal.
+       cbn. omega. eapply in_mm_sss_dec_0.
+
+       destruct (gt_0_eq (vec_pos v1 p0)); try omega.
+       eapply qs_encode_state with (i := i1 + 1) in H. destruct H1.
+       destruct H.
+       exists x. ring_simplify. repeat rewrite <- mult_assoc. rewrite <- H.
+       unfold encode_state, fst, snd. ring.
+     * eapply IHP in H7. subst.
+       destruct H7 as (k & l & [ u | u j ] & r & v & ? & ? & ?).
+       -- inv H. inv H0. inv H2.
+          exists i. exists (DEC p0 n :: l). exists (INC u). exists r. exists v.
+          cbn. repeat split. f_equal. omega.
+          econstructor.
+       -- inv H. inv H0. inv H2.
+          ++ exists i. exists (DEC p0 n :: l). exists (DEC u i2). exists r. exists v2.
+             cbn. repeat split. f_equal. omega.
+             econstructor. eauto.
+          ++ exists i. exists (DEC p0 n :: l). exists (DEC u j). exists r. exists v.
+             cbn. repeat split. f_equal. omega.
+             econstructor. eauto.
+       -- eauto.
+Qed.
+
+Lemma step_inv m i P i1 (v1 : vec nat m) st :
+     @mm_no_self_loops m (i,P) 
+  -> encode_mm_instr i P /F/ encode_state (i1,v1) → st 
+  -> exists i2 v2, st = @encode_state m (i2,v2).
+Proof with eauto; try omega.
+  intros HP ?. revert i H HP. induction P; intros i H0 HP.
+  - cbn in H0. inv H0.
+  - cbn in H0. inv H0.
+    + destruct a; inv H.
+      * exists (i + 1), (vec_change v1 p0 (S (v1 #> p0))).
+        unfold encode_state in H1.
+        assert (i = i1) as ->. {
+          match type of H1 with _ = ?r => assert (divides (ps i) r) end.
+          rewrite <- H1. exists st. ring.
+          eapply divides_mult_inv in H as [ [|] % divides_mult_inv | [|] % divides_mult_inv ]...
+          + eapply primestream_divides in H...
+          + eapply ps_qs_div in H...
+          + eapply primestream_divides in H...
+          + eapply ps_exp in H...
+        } unfold fst, snd in *; ring_simplify  in H1.
+        factorout H1 (ps i1). subst.
+        unfold encode_state, fst, snd. rewrite vec_prod_mult. replace (p0 + 0) with (0 + p0) by omega.
+        cbn. ring.
+      * unfold encode_state, fst, snd in H1.
+        assert (i = i1) as ->. {
+          match type of H1 with _ = ?r => assert (divides (ps i) r) end.
+          rewrite <- H1. exists (qs p0 * st). ring.
+          eapply divides_mult_inv in H as [ | [|] % divides_mult_inv ]...
+          + eapply primestream_divides in H...
+          + eapply primestream_divides in H...
+          + eapply ps_exp in H...
+        } 
+        factorout H1 (ps i1).
+
+        assert (v1 #> p0 > 0). {
+          eapply qs_encode_state.
+          match type of H1 with _ = ?r => assert (divides (qs p0) r) end.
+          rewrite <- H1. exists st. ring. eapply H.
+        }
+        destruct (v1 #> p0) eqn:E. inv H.
+        
+        exists (i1+1), (vec_change v1 p0 n0).
+        eapply Nat.mul_cancel_l. 2:rewrite H1. eauto.
+        unfold encode_state, fst, snd. ring_simplify.
+        rewrite <- !mult_assoc. rewrite Nat.mul_cancel_l. 2:eauto.
+        rewrite <- (vec_prod_div _ _ _ E). replace (p0 + 0) with (0 + p0) by omega.
+        cbn. ring.
+    + destruct a; inv H.
+      * eapply IHP in H2...
+      * inv H2.
+        -- unfold encode_state, fst, snd in H6.
+           assert (i = i1) as ->. {
+             match type of H6 with _ = ?r => assert (divides (ps i) r) end.
+             rewrite <- H6. exists st. ring.
+             eapply divides_mult_inv in H as [  | [|] % divides_mult_inv ]...
+             + eapply primestream_divides in H. subst. destruct (HP n p0)...
+             + eapply primestream_divides in H...
+             + eapply ps_exp in H...
+           } 
+           factorout H6 (ps i1). subst.
+           unfold encode_state, fst, snd. eexists; eauto.
+        -- eapply IHP in H7...
+Qed.
+
+Lemma step_backward m i P i1 v1 st :
+     @mm_no_self_loops m (i, P)
+  -> encode_mm_instr i P /F/ @encode_state m (i1,v1) → st 
+  -> exists i2 v2, st = @encode_state m (i2,v2)
+                /\ (i, P) /MM/ (i1, v1) → (i2,v2).
+Proof.
+  intros H1 H2.
+   destruct step_inv with (2 := H2)
+        as (i2 & v2 & ->); auto.
+   apply one_step_backward in H2; eauto.
+Qed.
+
+Lemma steps_backward m i P i1 v1 k st :
+     @mm_no_self_loops m (i, P)
+  ->               encode_mm_instr i P /F/ encode_state (i1,v1) -[k]-> st 
+  -> exists i2 v2, (i, P) /MM/ (i1, v1) -[k]-> (i2,v2)
+                /\ st = encode_state (i2,v2). 
+Proof.
+  intros H1.
+  revert i1 v1 st; induction k as [ | k IHk ]; intros i1 v1 st H; simpl in H.
+  - subst; exists i1, v1; split; auto; constructor.
+  - destruct H as (st1 & H2 & H3).
+    destruct step_backward with (2 := H2)
+      as (i2 & v2 & -> & H5); auto.
+    destruct IHk with (1 := H3) as (i3 & v3 & ? & ->).
+    exists i3, v3; split; auto.
+    constructor 2 with (i2,v2); auto.
+Qed.
+
+(** DLW: I did rewrite that proof to be sure I did not miss
+    an argument for the paper *)
+
+Theorem mm_fractran_simulation n P v :
+     @mm_no_self_loops n (1, P) 
+  -> (1,P) /MM/ (1,v) ↓ <-> encode_mm_instr 1 P /F/ ps 1 * exp 0 v ↓.
+Proof.
+  intros HP.
+  change (ps 1* exp 0 v) with (encode_state (1,v)).
+  split.
+  + intros ((j,w) & (k & H1) & H2); simpl fst in *.
+    exists (encode_state (j,w)); split.
+    * exists k; apply steps_forward in H1; auto.
+    * intros x Hx.
+      destruct step_backward with (2 := Hx)
+        as (i2 & v2 & -> & ?); auto.
+      revert H; apply sss_out_step_stall; auto.
+  + intros (st & (k & H1) & H2).
+    destruct steps_backward with (2 := H1)
+      as (i2 & v2 & H3 & ->); auto.
+    exists (i2,v2); split.
+    * exists k; auto.
+    * simpl fst.
+      destruct (in_out_code_dec i2 (1,P)) as [ H4 | H4 ]; auto; exfalso.
+      destruct in_code_subcode with (1 := H4) as (rho & l & r & G1 & G2).
+      destruct (mm_sss_total rho (i2,v2)) as ((i3,v3) & G3).
+      apply H2 with (encode_state (i3,v3)).
+      apply one_step_forward; auto.
+      subst P; apply in_sss_step; auto.
+Qed.
+
+Theorem mm_fractran_n n (P : list (mm_instr n)) : 
+        { l |  Forall (fun c => snd c <> 0) l
+            /\ forall v, (1,P) /MM/ (1,v) ↓ <-> l /F/ ps 1 * exp 1 v ↓ }.
+Proof.
+   destruct mm_remove_self_loops with (P := P) as (Q & H1 & _ & H2).
+   exists (encode_mm_instr 1 Q); split. 
+   + generalize (encode_mm_instr_regular 1 Q); apply Forall_impl; intros; tauto.
+   + intros x.
+     rewrite H2, mm_fractran_simulation; auto.
+     simpl exp; rewrite Nat.add_0_r; tauto.
+Qed.
+
+Theorem mm_fractran n (P : list (mm_instr (S n))) : 
+     { l | forall x, (1,P) /MM/ (1,x##vec_zero) ↓ <-> l /F/ ps 1 * qs 1^x ↓ }.
+Proof.
+   destruct mm_fractran_n with (P := P) as (l & _ & Hl).
+   exists l; intros x; rewrite Hl; simpl.
+   rewrite exp_zero, Nat.mul_1_r; tauto.
+Qed.
