H10/HALT_MM.v
@@ -1,0 +1,28 @@
+(**************************************************************)
+(*   Copyright Dominique Larchey-Wendling [*]                 *)
+(*                                                            *)
+(*                             [*] Affiliation LORIA -- CNRS  *)
+(**************************************************************)
+(*      This file is distributed under the terms of the       *)
+(*         CeCILL v2 FREE SOFTWARE LICENSE AGREEMENT          *)
+(**************************************************************)
+
+Require Import ILL.Definitions.
+
+Require Import utils_tac pos vec mm_defs.
+
+Require Import UNDEC.
+
+From Undecidability.PCP Require Import singleTM TM_SRH SRH_SR SR_MPCP MPCP_PCP.
+
+Set Implicit Arguments.
+
+Corollary MM_HALTING_undec : Halt ⪯ MM_HALTING.
+Proof.
+  eapply reduces_transitive. exact TM_SRH.Halt_SRH.
+  eapply reduces_transitive. exact SRH_SR.reduction.
+  eapply reduces_transitive. exact SR_MPCP.reduction.
+  eapply reduces_transitive. exact MPCP_PCP.reduction.
+  exact PCP_MM_HALTING.
+Qed.
+
