ILL/MM_EILL.v
@@ -26,7 +26,7 @@ Section MM_HALTING_EILL_PROVABILITY.
     exact (Sig (1,P) 0, vec_map_list v (fun p : pos n => pos2nat p), 2 * n + 1).
   Defined.
 
-  Theorem MM_HALTING_EILL_PROVABILITY : MM_HALTING ⪯ EILL_PROVABILITY.
+  Theorem MM_HALTS_ON_ZERO_EILL_PROVABILITY : MM_HALTS_ON_ZERO ⪯ EILL_PROVABILITY.
   Proof.
     exists f.
     intros (n & P & v); simpl.
